update model for non-blocking assignment

verilog_src/pipeline/agp32_processor.sv
@@ -19,13 +19,20 @@ module agp32_processor(
 );
 
 logic[2:0] state = 3'd3;
-logic[63:0][31:0] R = '0;
+logic[63:0][31:0]R = '0;
 logic[31:0] acc_arg = 'x;
 logic acc_arg_ready = 0;
 logic do_interrupt = 0;
 logic[31:0] acc_res = 'x;
 logic acc_res_ready = 'x;
 logic[1:0] acc_state = 'x;
+logic[32:0] ALU_sum = 'x;
+logic[63:0] ALU_prod = 'x;
+logic[31:0] ALU_sub = 'x;
+logic[31:0] shift_sh = 'x;
+logic checkA = 'x;
+logic checkB = 'x;
+logic checkW = 'x;
 logic[31:0] IF_PC_input = 'x;
 logic[31:0] IF_instr = 'x;
 logic IF_PC_write_enable = 'x;
@@ -125,13 +132,99 @@ logic WB_state_flag = 'x;
 logic WB_enable = 0;
 logic[2:0] WB_data_sel = 'x;
 logic[5:0] WB_addrW = 'x;
-logic[5:0] WB_opc;
+logic[5:0] WB_opc = 'x;
 
-logic checkW,checkB,checkA;
-logic [31:0] shift_sh,input1,input2,ALU_sub;
-logic [3:0] func;
-logic [33:0] ALU_sum;
-logic [63:0] ALU_prod;
+always_comb begin
+if ((state == 3'd3) || (state == 3'd5)) begin
+IF_PC_write_enable = 0;
+ID_ID_write_enable = 0;
+ID_flush_flag = 1;
+ID_EX_write_enable = 0;
+EX_NOP_flag = 0;
+MEM_state_flag = 0;
+MEM_NOP_flag = 0;
+WB_state_flag = 0;
+end else begin
+if ((state == 3'd2) || ((state == 3'd4) || ((state == 3'd6) || (state == 3'd7)))) begin
+IF_PC_write_enable = 0;
+ID_ID_write_enable = 0;
+ID_flush_flag = 0;
+ID_EX_write_enable = 0;
+EX_NOP_flag = 0;
+MEM_state_flag = 0;
+MEM_NOP_flag = 0;
+WB_state_flag = 0;
+end else begin
+if (state == 3'd1) begin
+IF_PC_write_enable = 0;
+ID_ID_write_enable = 0;
+ID_flush_flag = 1;
+ID_EX_write_enable = 0;
+EX_NOP_flag = 0;
+MEM_state_flag = 1;
+MEM_NOP_flag = 0;
+WB_state_flag = 1;
+end else begin
+if (!ready) begin
+IF_PC_write_enable = 0;
+ID_ID_write_enable = 0;
+ID_flush_flag = 0;
+ID_EX_write_enable = 0;
+EX_NOP_flag = 0;
+MEM_state_flag = 0;
+MEM_NOP_flag = 0;
+WB_state_flag = 0;
+end else begin
+if ((MEM_opc == 6'd2) || ((MEM_opc == 6'd3) || ((MEM_opc == 6'd4) || ((MEM_opc == 6'd5) || (MEM_opc == 6'd12))))) begin
+IF_PC_write_enable = 0;
+ID_ID_write_enable = 0;
+ID_flush_flag = 0;
+ID_EX_write_enable = 0;
+EX_NOP_flag = 0;
+MEM_state_flag = 0;
+MEM_NOP_flag = 1;
+WB_state_flag = 1;
+end else begin
+if (!(PC_sel == 2'd0)) begin
+IF_PC_write_enable = 1;
+ID_ID_write_enable = 0;
+ID_flush_flag = 1;
+ID_EX_write_enable = 1;
+EX_NOP_flag = 1;
+MEM_state_flag = 1;
+MEM_NOP_flag = 0;
+WB_state_flag = 1;
+end else begin
+IF_PC_write_enable = 1;
+ID_ID_write_enable = 1;
+ID_flush_flag = 0;
+ID_EX_write_enable = 1;
+EX_NOP_flag = 0;
+MEM_state_flag = 1;
+MEM_NOP_flag = 0;
+WB_state_flag = 1;
+end
+end
+end
+end
+end
+end
+end
+
+always_comb begin
+checkA = (EX_opc == 6'd0) || ((EX_opc == 6'd1) || ((EX_opc == 6'd2) || ((EX_opc == 6'd3) || ((EX_opc == 6'd4) || ((EX_opc == 6'd5) || ((EX_opc == 6'd6) || ((EX_opc == 6'd8) || ((EX_opc == 6'd9) || ((EX_opc == 6'd10) || (EX_opc == 6'd11))))))))));
+EX_ForwardA = ((EX_addrA == MEM_addrW) && (MEM_write_reg && (((MEM_opc == 6'd13) || (MEM_opc == 6'd14)) && ((!EX_addrA_enable) && checkA)))) ? 3'd5 : (((EX_addrA == MEM_addrW) && (MEM_write_reg && ((MEM_opc == 6'd9) && ((!EX_addrA_enable) && checkA)))) ? 3'd4 : (((EX_addrA == MEM_addrW) && (MEM_write_reg && ((MEM_opc == 6'd1) && ((!EX_addrA_enable) && checkA)))) ? 3'd3 : (((EX_addrA == MEM_addrW) && (MEM_write_reg && (((MEM_opc == 6'd0) || (MEM_opc == 6'd6)) && ((!EX_addrA_enable) && checkA)))) ? 3'd2 : (((EX_addrA == WB_addrW) && (WB_write_reg && ((!EX_addrA_enable) && checkA))) ? 3'd1 : 3'd0))));
+end
+
+always_comb begin
+checkB = (EX_opc == 6'd0) || ((EX_opc == 6'd1) || ((EX_opc == 6'd2) || ((EX_opc == 6'd3) || ((EX_opc == 6'd6) || ((EX_opc == 6'd10) || (EX_opc == 6'd11))))));
+EX_ForwardB = ((EX_addrB == MEM_addrW) && (MEM_write_reg && (((MEM_opc == 6'd13) || (MEM_opc == 6'd14)) && ((!EX_addrB_enable) && checkB)))) ? 3'd5 : (((EX_addrB == MEM_addrW) && (MEM_write_reg && ((MEM_opc == 6'd9) && ((!EX_addrB_enable) && checkB)))) ? 3'd4 : (((EX_addrB == MEM_addrW) && (MEM_write_reg && ((MEM_opc == 6'd1) && ((!EX_addrB_enable) && checkB)))) ? 3'd3 : (((EX_addrB == MEM_addrW) && (MEM_write_reg && (((MEM_opc == 6'd0) || (MEM_opc == 6'd6)) && ((!EX_addrB_enable) && checkB)))) ? 3'd2 : (((EX_addrB == WB_addrW) && (WB_write_reg && ((!EX_addrB_enable) && checkB))) ? 3'd1 : 3'd0))));
+end
+
+always_comb begin
+checkW = (EX_opc == 6'd10) || ((EX_opc == 6'd11) || (EX_opc == 6'd14));
+EX_ForwardW = ((EX_addrW == MEM_addrW) && (MEM_write_reg && (((MEM_opc == 6'd13) || (MEM_opc == 6'd14)) && ((!EX_addrW_enable) && checkW)))) ? 3'd5 : (((EX_addrW == MEM_addrW) && (MEM_write_reg && ((MEM_opc == 6'd9) && ((!EX_addrW_enable) && checkW)))) ? 3'd4 : (((EX_addrW == MEM_addrW) && (MEM_write_reg && ((MEM_opc == 6'd1) && ((!EX_addrW_enable) && checkW)))) ? 3'd3 : (((EX_addrW == MEM_addrW) && (MEM_write_reg && (((MEM_opc == 6'd0) || (MEM_opc == 6'd6)) && ((!EX_addrW_enable) && checkW)))) ? 3'd2 : (((EX_addrW == WB_addrW) && (WB_write_reg && ((!EX_addrW_enable) && checkW))) ? 3'd1 : 3'd0))));
+end
 
 always_comb begin
 IF_instr = ready ? inst_rdata : 32'd63;
@@ -139,102 +232,10 @@ end
 
 always_comb begin
 if ((EX_PC_sel == 2'd1) || (((EX_PC_sel == 2'd2) && (EX_ALU_res == 32'd0)) || ((EX_PC_sel == 2'd3) && (!(EX_ALU_res == 32'd0))))) begin
-PC_sel <= EX_PC_sel;
+PC_sel = EX_PC_sel;
 end else begin
-PC_sel <= 2'd0;
+PC_sel = 2'd0;
 end
-end
-
-always_comb begin
-if ((state == 3'd3) || (state == 3'd5)) begin
-IF_PC_write_enable = 0;
-ID_ID_write_enable = 0;
-ID_flush_flag = 1;
-ID_EX_write_enable <= 0;
-EX_NOP_flag = 0;
-MEM_state_flag <= 0;
-MEM_NOP_flag = 0;
-WB_state_flag <= 0;
-end else begin
-if ((state == 3'd2) || ((state == 3'd4) || ((state == 3'd6) || (state == 3'd7)))) begin
-IF_PC_write_enable = 0;
-ID_ID_write_enable = 0;
-ID_flush_flag = 0;
-ID_EX_write_enable <= 0;
-EX_NOP_flag = 0;
-MEM_state_flag <= 0;
-MEM_NOP_flag = 0;
-WB_state_flag <= 0;
-end else begin
-if (state == 3'd1) begin
-IF_PC_write_enable = 0;
-ID_ID_write_enable = 0;
-ID_flush_flag = 1;
-ID_EX_write_enable <= 0;
-EX_NOP_flag = 0;
-MEM_state_flag <= 1;
-MEM_NOP_flag = 0;
-WB_state_flag <= 1;
-end else begin
-if (!ready) begin
-IF_PC_write_enable = 0;
-ID_ID_write_enable = 0;
-ID_flush_flag = 0;
-ID_EX_write_enable <= 0;
-EX_NOP_flag = 0;
-MEM_state_flag <= 0;
-MEM_NOP_flag = 0;
-WB_state_flag <= 0;
-end else begin
-if ((MEM_opc == 6'd2) || ((MEM_opc == 6'd3) || ((MEM_opc == 6'd4) || ((MEM_opc == 6'd5) || (MEM_opc == 6'd12))))) begin
-IF_PC_write_enable = 0;
-ID_ID_write_enable = 0;
-ID_flush_flag = 0;
-ID_EX_write_enable <= 0;
-EX_NOP_flag = 0;
-MEM_state_flag <= 0;
-MEM_NOP_flag = 1;
-WB_state_flag <= 1;
-end else begin
-if (!(PC_sel == 2'd0)) begin
-IF_PC_write_enable = 1;
-ID_ID_write_enable = 0;
-ID_flush_flag = 1;
-ID_EX_write_enable <= 1;
-EX_NOP_flag = 1;
-MEM_state_flag <= 1;
-MEM_NOP_flag = 0;
-WB_state_flag <= 1;
-end else begin
-IF_PC_write_enable = 1;
-ID_ID_write_enable = 1;
-ID_flush_flag = 0;
-ID_EX_write_enable <= 1;
-EX_NOP_flag = 0;
-MEM_state_flag <= 1;
-MEM_NOP_flag = 0;
-WB_state_flag <= 1;
-end
-end
-end
-end
-end
-end
-end
-
-always_comb begin
-checkW = (EX_opc == 6'd10) || ((EX_opc == 6'd11) || (EX_opc == 6'd14));
-EX_ForwardW <= ((EX_addrW == MEM_addrW) && (MEM_write_reg && (((MEM_opc == 6'd13) || (MEM_opc == 6'd14)) && ((!EX_addrW_enable) && checkW)))) ? 3'd5 : (((EX_addrW == MEM_addrW) && (MEM_write_reg && ((MEM_opc == 6'd9) && ((!EX_addrW_enable) && checkW)))) ? 3'd4 : (((EX_addrW == MEM_addrW) && (MEM_write_reg && ((MEM_opc == 6'd1) && ((!EX_addrW_enable) && checkW)))) ? 3'd3 : (((EX_addrW == MEM_addrW) && (MEM_write_reg && (((MEM_opc == 6'd0) || (MEM_opc == 6'd6)) && ((!EX_addrW_enable) && checkW)))) ? 3'd2 : (((EX_addrW == WB_addrW) && (WB_write_reg && ((!EX_addrW_enable) && checkW))) ? 3'd1 : 3'd0))));
-end
-
-always_comb begin
-checkB = (EX_opc == 6'd0) || ((EX_opc == 6'd1) || ((EX_opc == 6'd2) || ((EX_opc == 6'd3) || ((EX_opc == 6'd6) || ((EX_opc == 6'd10) || (EX_opc == 6'd11))))));
-EX_ForwardB <= ((EX_addrB == MEM_addrW) && (MEM_write_reg && (((MEM_opc == 6'd13) || (MEM_opc == 6'd14)) && ((!EX_addrB_enable) && checkB)))) ? 3'd5 : (((EX_addrB == MEM_addrW) && (MEM_write_reg && ((MEM_opc == 6'd9) && ((!EX_addrB_enable) && checkB)))) ? 3'd4 : (((EX_addrB == MEM_addrW) && (MEM_write_reg && ((MEM_opc == 6'd1) && ((!EX_addrB_enable) && checkB)))) ? 3'd3 : (((EX_addrB == MEM_addrW) && (MEM_write_reg && (((MEM_opc == 6'd0) || (MEM_opc == 6'd6)) && ((!EX_addrB_enable) && checkB)))) ? 3'd2 : (((EX_addrB == WB_addrW) && (WB_write_reg && ((!EX_addrB_enable) && checkB))) ? 3'd1 : 3'd0))));
-end
-
-always_comb begin
-checkA = (EX_opc == 6'd0) || ((EX_opc == 6'd1) || ((EX_opc == 6'd2) || ((EX_opc == 6'd3) || ((EX_opc == 6'd4) || ((EX_opc == 6'd5) || ((EX_opc == 6'd6) || ((EX_opc == 6'd8) || ((EX_opc == 6'd9) || ((EX_opc == 6'd10) || (EX_opc == 6'd11))))))))));
-EX_ForwardA <= ((EX_addrA == MEM_addrW) && (MEM_write_reg && (((MEM_opc == 6'd13) || (MEM_opc == 6'd14)) && ((!EX_addrA_enable) && checkA)))) ? 3'd5 : (((EX_addrA == MEM_addrW) && (MEM_write_reg && ((MEM_opc == 6'd9) && ((!EX_addrA_enable) && checkA)))) ? 3'd4 : (((EX_addrA == MEM_addrW) && (MEM_write_reg && ((MEM_opc == 6'd1) && ((!EX_addrA_enable) && checkA)))) ? 3'd3 : (((EX_addrA == MEM_addrW) && (MEM_write_reg && (((MEM_opc == 6'd0) || (MEM_opc == 6'd6)) && ((!EX_addrA_enable) && checkA)))) ? 3'd2 : (((EX_addrA == WB_addrW) && (WB_write_reg && ((!EX_addrA_enable) && checkA))) ? 3'd1 : 3'd0))));
 end
 
 always_comb begin
@@ -267,14 +268,12 @@ end
 end
 end
 end
-
 if ((ID_opc == 6'd0) || ((ID_opc == 6'd1) || ((ID_opc == 6'd6) || ((ID_opc == 6'd9) || ((ID_opc == 6'd10) || (ID_opc == 6'd11)))))) begin
 ID_func = ID_instr[9:6];
 end else begin
 ID_func = 4'd9;
 end
 end
-
 
 always_comb begin
 if (ID_instr[31] && ID_instr[24]) begin
@@ -292,7 +291,6 @@ end
 end
 end
 
-
 always_comb begin
 ID_addrA = ID_instr[22:17];
 ID_addrB = ID_instr[15:10];
@@ -300,23 +298,18 @@ ID_addrW = ID_instr[30:25];
 ID_addrA_enable = ID_instr[23];
 ID_addrB_enable = ID_instr[16];
 ID_addrW_enable = ID_instr[31];
-
 ID_read_dataA = R[ID_addrA];
 ID_read_dataB = R[ID_addrB];
 ID_read_dataW = R[ID_addrW];
-
 ID_immA = {32'($signed(ID_instr[22:17]))};
 ID_immB = {32'($signed(ID_instr[15:10]))};
 ID_immW = {32'($signed(ID_instr[30:25]))};
-
 ID_ForwardA = ((ID_addrA == WB_addrW) && (WB_write_reg && WB_state_flag)) ? 1 : 0;
 ID_ForwardB = ((ID_addrB == WB_addrW) && (WB_write_reg && WB_state_flag)) ? 1 : 0;
 ID_ForwardW = ((ID_addrW == WB_addrW) && (WB_write_reg && WB_state_flag)) ? 1 : 0;
-
 ID_read_dataA_updated = ID_ForwardA ? WB_write_data : ID_read_dataA;
 ID_read_dataB_updated = ID_ForwardB ? WB_write_data : ID_read_dataB;
 ID_read_dataW_updated = ID_ForwardW ? WB_write_data : ID_read_dataW;
-
 ID_dataA = ID_instr[23] ? ID_immA : ID_read_dataA_updated;
 ID_dataB = ID_instr[16] ? ID_immB : ID_read_dataB_updated;
 ID_dataW = ID_instr[31] ? ID_immW : ID_read_dataW_updated;
@@ -325,7 +318,7 @@ end
 always_comb begin
 if (ID_EX_write_enable) begin
 EX_isAcc = EX_opc == 6'd8;
-EX_PC_sel <= (EX_opc == 6'd9) ? 2'd1 : ((EX_opc == 6'd10) ? 2'd2 : ((EX_opc == 6'd11) ? 2'd3 : 2'd0));
+EX_PC_sel = (EX_opc == 6'd9) ? 2'd1 : ((EX_opc == 6'd10) ? 2'd2 : ((EX_opc == 6'd11) ? 2'd3 : 2'd0));
 end
 end
 
@@ -333,12 +326,54 @@ always_comb begin
 EX_dataA_updated = (EX_ForwardA == 3'd0) ? EX_dataA : ((EX_ForwardA == 3'd1) ? WB_write_data : ((EX_ForwardA == 3'd2) ? MEM_ALU_res : ((EX_ForwardA == 3'd3) ? MEM_SHIFT_res : ((EX_ForwardA == 3'd4) ? (MEM_PC + 32'd4) : ((EX_ForwardA == 3'd5) ? MEM_imm_updated : ((EX_ForwardA == 3'd6) ? 32'd0 : 32'd0))))));
 EX_dataB_updated = (EX_ForwardB == 3'd0) ? EX_dataB : ((EX_ForwardB == 3'd1) ? WB_write_data : ((EX_ForwardB == 3'd2) ? MEM_ALU_res : ((EX_ForwardB == 3'd3) ? MEM_SHIFT_res : ((EX_ForwardB == 3'd4) ? (MEM_PC + 32'd4) : ((EX_ForwardB == 3'd5) ? MEM_imm_updated : ((EX_ForwardB == 3'd6) ? 32'd0 : 32'd0))))));
 EX_dataW_updated = (EX_ForwardW == 3'd0) ? EX_dataW : ((EX_ForwardW == 3'd1) ? WB_write_data : ((EX_ForwardW == 3'd2) ? MEM_ALU_res : ((EX_ForwardW == 3'd3) ? MEM_SHIFT_res : ((EX_ForwardW == 3'd4) ? (MEM_PC + 32'd4) : ((EX_ForwardW == 3'd5) ? MEM_imm_updated : ((EX_ForwardW == 3'd6) ? 32'd0 : 32'd0))))));
+end
 
+always_comb begin
 EX_ALU_input1 = (EX_opc == 6'd9) ? EX_PC : EX_dataA_updated;
 EX_ALU_input2 = (EX_opc == 6'd9) ? EX_dataA_updated : EX_dataB_updated;
+end
 
+always_comb begin
 EX_compute_enable = (state == 3'd0) && ((!(MEM_opc == 6'd16)) || ((MEM_opc == 6'd16) && ((!(EX_ForwardA == 3'd0)) || (!(EX_ForwardB == 3'd0)))));
+end
 
+always_comb begin
+ALU_sum = (33'({EX_ALU_input1}) + 33'({EX_ALU_input2})) + ((EX_func == 4'd1) ? 33'({EX_carry_flag}) : 33'd0);
+ALU_prod = 64'({EX_ALU_input1}) * 64'({EX_ALU_input2});
+if (EX_compute_enable) begin
+case (EX_func)
+4'd0 : begin
+EX_overflow_flag = (EX_ALU_input1[31] == EX_ALU_input2[31]) && (!(ALU_sum[31] == EX_ALU_input1[31]));
+EX_carry_flag = ALU_sum[32];
+EX_ALU_res = ALU_sum[31:0];
+end
+4'd1 : begin
+EX_carry_flag = ALU_sum[32];
+EX_ALU_res = ALU_sum[31:0];
+end
+4'd2 : begin
+ALU_sub = EX_ALU_input1 - EX_ALU_input2;
+EX_ALU_res = ALU_sub;
+EX_overflow_flag = (!(EX_ALU_input1[31] == EX_ALU_input2[31])) && (!(ALU_sub[31] == EX_ALU_input1[31]));
+end
+4'd3 : EX_ALU_res = 32'({EX_carry_flag});
+4'd4 : EX_ALU_res = 32'({EX_overflow_flag});
+4'd5 : EX_ALU_res = EX_ALU_input1 + 32'd1;
+4'd6 : EX_ALU_res = EX_ALU_input1 - 32'd1;
+4'd7 : EX_ALU_res = ALU_prod[31:0];
+4'd8 : EX_ALU_res = ALU_prod[63:32];
+4'd9 : EX_ALU_res = EX_ALU_input1 & EX_ALU_input2;
+4'd10 : EX_ALU_res = EX_ALU_input1 | EX_ALU_input2;
+4'd11 : EX_ALU_res = EX_ALU_input1 ^^ EX_ALU_input2;
+4'd12 : EX_ALU_res = 32'({EX_ALU_input1 == EX_ALU_input2});
+4'd13 : EX_ALU_res = 32'({{$signed(EX_ALU_input1) < $signed(EX_ALU_input2)}});
+4'd14 : EX_ALU_res = 32'({EX_ALU_input1 < EX_ALU_input2});
+4'd15 : EX_ALU_res = EX_ALU_input2;
+endcase
+end
+end
+
+always_comb begin
 if (EX_compute_enable) begin
 case (EX_func[1:0])
 2'd0 : EX_SHIFT_res = EX_dataA_updated << EX_dataB_updated;
@@ -350,53 +385,18 @@ EX_SHIFT_res = (EX_dataA_updated >> shift_sh) | (EX_dataA_updated << (32'd32 - s
 end
 endcase
 end
-
-input1 = EX_ALU_input1;
-input2 = EX_ALU_input2;
-func = EX_func;
-ALU_sum = (33'({input1}) + 33'({input2})) + ((func == 4'd1) ? 33'({EX_carry_flag}) : 33'd0);
-ALU_prod = 64'({input1}) * 64'({input2});
-if (EX_compute_enable) begin
-case (func)
-4'd0 : begin
-EX_overflow_flag = (input1[31] == input2[31]) && (!(ALU_sum[31] == input1[31]));
-EX_carry_flag = ALU_sum[32];
-EX_ALU_res = ALU_sum[31:0];
-end
-4'd1 : begin
-EX_carry_flag = ALU_sum[32];
-EX_ALU_res = ALU_sum[31:0];
-end
-4'd2 : begin
-ALU_sub = input1 - input2;
-EX_ALU_res = ALU_sub;
-EX_overflow_flag = (!(input1[31] == input2[31])) && (!(ALU_sub[31] == input1[31]));
-end
-4'd3 : EX_ALU_res = 32'({EX_carry_flag});
-4'd4 : EX_ALU_res = 32'({EX_overflow_flag});
-4'd5 : EX_ALU_res = input1 + 32'd1;
-4'd6 : EX_ALU_res = input1 - 32'd1;
-4'd7 : EX_ALU_res = ALU_prod[31:0];
-4'd8 : EX_ALU_res = ALU_prod[63:32];
-4'd9 : EX_ALU_res = input1 & input2;
-4'd10 : EX_ALU_res = input1 | input2;
-4'd11 : EX_ALU_res = input1 ^^ input2;
-4'd12 : EX_ALU_res = 32'({input1 == input2});
-4'd13 : EX_ALU_res = 32'({{$signed(input1) < $signed(input2)}});
-4'd14 : EX_ALU_res = 32'({input1 < input2});
-4'd15 : EX_ALU_res = input2;
-endcase
 end
 
+always_comb begin
 if ((state == 3'd0) && (!(MEM_opc == 6'd16))) begin
 EX_dataA_rec = EX_dataA_updated;
 EX_dataB_rec = EX_dataB_updated;
 EX_dataW_rec = EX_dataW_updated;
 end else begin
 if ((state == 3'd0) && (MEM_opc == 6'd16)) begin
-if (!(EX_ForwardA == 3'd0)) EX_dataA_rec = EX_dataA_updated;
-if (!(EX_ForwardB == 3'd0)) EX_dataB_rec = EX_dataB_updated;
-if (!(EX_ForwardW == 3'd0)) EX_dataW_rec = EX_dataW_updated;
+EX_dataA_rec = (!(EX_ForwardA == 3'd0)) ? EX_dataA_updated : EX_dataA_rec;
+EX_dataB_rec = (!(EX_ForwardB == 3'd0)) ? EX_dataB_updated : EX_dataB_rec;
+EX_dataW_rec = (!(EX_ForwardW == 3'd0)) ? EX_dataW_updated : EX_dataW_rec;
 end
 end
 end
@@ -406,27 +406,22 @@ if ((EX_write_enable && MEM_state_flag) || MEM_enable) begin
 MEM_read_mem = (MEM_opc == 6'd4) || (MEM_opc == 6'd5);
 MEM_write_mem = MEM_opc == 6'd2;
 MEM_write_mem_byte = MEM_opc == 6'd3;
-//MEM_write_reg = (MEM_opc == 6'd0) || ((MEM_opc == 6'd1) || ((MEM_opc == 6'd4) || ((MEM_opc == 6'd5) || ((MEM_opc == 6'd6) || ((MEM_opc == 6'd7) || ((MEM_opc == 6'd8) || ((MEM_opc == 6'd9) || ((MEM_opc == 6'd13) || (MEM_opc == 6'd14)))))))));
 MEM_isInterrupt = MEM_opc == 6'd12;
 end
 end
 
 always_comb begin
-MEM_imm_updated <= (MEM_opc == 6'd14) ? {MEM_imm[8:0], MEM_dataW[22:0]} : MEM_imm;
+MEM_imm_updated = (MEM_opc == 6'd14) ? {MEM_imm[8:0], MEM_dataW[22:0]} : MEM_imm;
 end
 
 always_comb begin
 WB_read_data = data_rdata;
-
+WB_read_data_byte = (WB_dataA[1:0] == 2'd0) ? 32'({WB_read_data[7:0]}) : ((WB_dataA[1:0] == 2'd1) ? 32'({WB_read_data[15:8]}) : ((WB_dataA[1:0] == 2'd2) ? 32'({WB_read_data[23:16]}) : 32'({WB_read_data[31:24]})));
 if ((MEM_write_enable && WB_state_flag) || WB_enable) begin
 WB_isOut = WB_opc == 6'd6;
 WB_data_sel = ((WB_opc == 6'd0) || (WB_opc == 6'd6)) ? 3'd0 : ((WB_opc == 6'd1) ? 3'd1 : ((WB_opc == 6'd7) ? 3'd2 : ((WB_opc == 6'd9) ? 3'd3 : (((WB_opc == 6'd13) || (WB_opc == 6'd14)) ? 3'd4 : ((WB_opc == 6'd4) ? 3'd5 : ((WB_opc == 6'd5) ? 3'd6 : ((WB_opc == 6'd8) ? 3'd7 : 3'd0)))))));
 end
-
-WB_read_data_byte = (WB_dataA[1:0] == 2'd0) ? 32'({WB_read_data[7:0]}) : ((WB_dataA[1:0] == 2'd1) ? 32'({WB_read_data[15:8]}) : ((WB_dataA[1:0] == 2'd2) ? 32'({WB_read_data[23:16]}) : 32'({WB_read_data[31:24]})));
-
-
-WB_write_data <= (WB_data_sel == 3'd0) ? WB_ALU_res : ((WB_data_sel == 3'd1) ? WB_SHIFT_res : ((WB_data_sel == 3'd2) ? 32'({data_in}) : ((WB_data_sel == 3'd3) ? (WB_PC + 32'd4) : ((WB_data_sel == 3'd4) ? WB_imm : ((WB_data_sel == 3'd5) ? WB_read_data : ((WB_data_sel == 3'd6) ? WB_read_data_byte : acc_res))))));
+WB_write_data = (WB_data_sel == 3'd0) ? WB_ALU_res : ((WB_data_sel == 3'd1) ? WB_SHIFT_res : ((WB_data_sel == 3'd2) ? 32'({data_in}) : ((WB_data_sel == 3'd3) ? (WB_PC + 32'd4) : ((WB_data_sel == 3'd4) ? WB_imm : ((WB_data_sel == 3'd5) ? WB_read_data : ((WB_data_sel == 3'd6) ? WB_read_data_byte : acc_res))))));
 end
 
 always_ff @ (posedge clk) begin
@@ -438,10 +433,10 @@ end
 always_ff @ (posedge clk) begin
 if (ID_ID_write_enable) begin
 ID_PC <= PC;
-ID_instr <= IF_instr;
+ID_instr = IF_instr;
 end else begin
 if (ID_flush_flag) begin
-ID_instr <= 32'd63;
+ID_instr = 32'd63;
 end
 end
 end
@@ -468,8 +463,7 @@ EX_addrB = ID_addrB;
 EX_addrW <= ID_addrW;
 EX_opc <= EX_NOP_flag ? 6'd16 : ID_opc;
 EX_func = ID_func;
-end
-else begin
+end else begin
 EX_write_enable <= 0;
 end
 end
@@ -480,18 +474,19 @@ MEM_PC <= EX_PC;
 MEM_dataA <= EX_dataA_rec;
 MEM_dataB <= EX_dataB_rec;
 MEM_dataW = EX_dataW_rec;
-MEM_imm <= EX_imm;
+MEM_imm = EX_imm;
 MEM_ALU_res <= EX_ALU_res;
 MEM_SHIFT_res <= EX_SHIFT_res;
 MEM_write_enable <= 1;
 MEM_addrW <= EX_addrW;
 MEM_opc <= EX_opc;
-MEM_write_reg <= (EX_opc == 6'd0) || ((EX_opc == 6'd1) || ((EX_opc == 6'd4) || ((EX_opc == 6'd5) || ((EX_opc == 6'd6) || ((EX_opc == 6'd7) || ((EX_opc == 6'd8) || ((EX_opc == 6'd9) || ((EX_opc == 6'd13) || (EX_opc == 6'd14)))))))));
-end
-else begin
+MEM_write_reg = (EX_opc == 6'd0) || ((EX_opc == 6'd1) || ((EX_opc == 6'd4) || ((EX_opc == 6'd5) || ((EX_opc == 6'd6) || ((EX_opc == 6'd7) || ((EX_opc == 6'd8) || ((EX_opc == 6'd9) || ((EX_opc == 6'd13) || (EX_opc == 6'd14)))))))));
+end else begin
 MEM_write_enable <= 0;
 end
-if (MEM_NOP_flag) begin MEM_opc <= 6'd16; end
+if (MEM_NOP_flag) begin
+MEM_opc <= 6'd16;
+end
 end
 
 always_ff @ (posedge clk) begin
@@ -501,8 +496,7 @@ WB_dataA = MEM_dataA;
 WB_imm = MEM_imm_updated;
 WB_ALU_res = MEM_ALU_res;
 WB_SHIFT_res = MEM_SHIFT_res;
-WB_write_reg <= (MEM_opc == 6'd0) || ((MEM_opc == 6'd1) || ((MEM_opc == 6'd4) || ((MEM_opc == 6'd5) || ((EX_opc == 6'd6) || ((MEM_opc == 6'd7) || ((MEM_opc == 6'd8) || ((MEM_opc == 6'd9) || ((MEM_opc == 6'd13) || (MEM_opc == 6'd14)))))))));
-;
+WB_write_reg <= (MEM_opc == 6'd0) || ((MEM_opc == 6'd1) || ((MEM_opc == 6'd4) || ((MEM_opc == 6'd5) || ((MEM_opc == 6'd6) || ((MEM_opc == 6'd7) || ((MEM_opc == 6'd8) || ((MEM_opc == 6'd9) || ((MEM_opc == 6'd13) || (MEM_opc == 6'd14)))))))));
 WB_addrW <= MEM_addrW;
 WB_opc = MEM_opc;
 end
