model/compilation/agp32VerilogScript.sml
@@ -12,13 +12,8 @@ local
                 "data_addr", "data_wdata", "data_wstrb"]
  val comms = ["data_out", "command", "data_addr", "data_wdata", "data_wstrb",
               "acc_arg", "acc_arg_ready", "acc_res", "acc_res_ready", "interrupt_req",
-              "PC_sel", "ID_EX_write_enable", "MEM_state_flag", "WB_state_flag",
-              "EX_ForwardA", "EX_ForwardB", "EX_ForwardW", "EX_PC_sel",
-              "EX_dataA_updated", "EX_dataB_updated", "EX_dataW_updated",
-              "EX_ALU_input1", "EX_ALU_input2", "EX_compute_enable",
-              "MEM_imm_updated", "WB_write_data", "PC", "ID_PC", "ID_instr", "EX_PC",
-              "EX_imm", "EX_write_enable", "EX_addrW", "EX_opc",
-              "MEM_PC", "MEM_dataA", "MEM_dataB", "MEM_ALU_res", "MEM_imm_updated",
+              "PC", "ID_PC", "EX_PC", "EX_imm", "EX_write_enable", "EX_addrW", "EX_opc",
+              "MEM_PC", "MEM_dataA", "MEM_dataB", "MEM_ALU_res",
               "MEM_SHIFT_res", "MEM_write_enable", "MEM_addrW", "MEM_opc",
               "WB_write_reg", "WB_addrW", "MEM_enable", "WB_enable"]
 in
